src/PlutusIR/Semantics/Dynamic/Bigstep/EvalValue.v
@@ -8,10 +8,15 @@ Lemma eval_value :
   (forall v, value v -> v =[0]=> v) /\
   (forall n v, neutral_value n v -> v =[0]=> v).
 Proof with (autounfold; (eauto || (try lia))).
-  apply value__multind.
+  apply value___multind.
   all: intros.
   all: try solve [constructor; eauto].
-  - inversion H; subst...
+  (* Constr*)
+  - induction vs.
+    + constructor.
+    + inversion H. inversion H0. subst.
+      eapply E_Constr_cons with (k_t := 0) (k_ts := 0)...
+  - assumption.
   - inversion H2; subst.
     all: econstructor...
     all: econstructor...
